Started bubble sort

UMap.dfy
@@ -15,14 +15,20 @@ import opened M = Map
 import opened Option
 
 class UMap<T(!new,==)> {
-
+  var entries : Map<T>
   // this.entrySet() is the set of all the entries in the map 
   ghost function entrySet(): set<Entry<T>>
     reads this
+    {
+      L.elements(entries)
+    }
 
   // this.keySet() is the set of all the keys in the map 
   ghost function keySet(): set<int>
     reads this
+    requires isValid()
+    ensures isEmpty() <==> keySet() == {}
+
   {
     M.keys(entries)
   }
@@ -30,6 +36,8 @@ class UMap<T(!new,==)> {
   // this.valueSet() is the set of all the values in the map 
   ghost function valueSet(): set<T>
     reads this
+    requires isValid()
+    ensures isEmpty() <==> valueSet() == {}
   {
     M.values(entries)
   }
@@ -45,42 +53,94 @@ class UMap<T(!new,==)> {
   // this.hasValue(k) is true iff key k as a value in the map
   ghost predicate hasValue(k: int)
     reads this
+    requires isValid()
+    {
+      k in keySet()
+    }
 
   // this.isEmpty() is true iff the map contains no entries
   predicate isEmpty() 
     reads this
+    requires isValid()
+    ensures isEmpty() <==> |entrySet()| == 0
+    {
+      M.isEmpty(entries)
+    }
 
 
   // constructor returns a (new) map with an empty set of entries.
   constructor ()
-    modifies this 
     ensures isValid()
     ensures entrySet() == {}
     ensures keySet() == {}
   {
-
+    entries := M.emptyMap();
   }
 
   // this.size() returns the number of entries in the map
   method size() returns (s: nat) 
-    ensures s == |entrySet()|
-    reads this
+    requires isValid()
+    ensures isEmpty() <==> s == 0
+    ensures !isEmpty() ==> s > 0
+    {
+      s := M.size(entries);
+    }
 
   // this.get(k) returns the value associated to key k in the map, if any.
   // More precisely, it returns Some(v) if k has an associated value v,
   // and returns None otherwhise.
   method get(k: int) returns (vo: Option<T>)
+   requires isValid()
+    ensures isValid()
+    ensures (vo ==  None) <==> k !in keySet()
+    // ensures (vo == None) <==> k !in keys2(m)
+    ensures (vo != None) ==> (k, vo.val) in entrySet()
+  
+  {
+    vo := M.get(entries, k);
+  }
 
 
   // this.put(k, v) changes the map so that key k is associated with value v.
   // Then it returns the value previously associated to k in the map, if any.
   // More precisely, it returns Some(v) if k had an associated value v,
   // and returns None otherwhise.
-  method put(k: int, v: T) returns (old_vo: Option<T>)
+  method put(k: int, v: T) returns (old_vo: Option<T>) 
+  requires isValid()
+  ensures isValid()
+  modifies this
+  ensures keySet() == old(keySet()) + {k}
+  ensures v in valueSet()
+  ensures (k, v) in entrySet()
+  ensures old_vo != None ==> (entrySet() - {(k,v)} 
+        <= old(entrySet()) )
+  ensures old_vo != None ==> (k, old_vo.val) in old(entrySet())
+  
+
+    // ensures forall q :: q != k ==> 
+    //     get(put(m,k,v), q) == get(m, q)
+
+    // ensures k in old(keySet()) ==> size(entrySet) == size(m) 
+    // ensures k !in keys(m) ==> size(put(m,k,v)) == size(m) + 1
+    // ensures values(put(m, k, v)) <= values(m) + {v}
+    {
+      old_vo := get(k);
+      entries := M.put(entries,k,v);
+    }
 
   // this.remove(k) removes from the map the entry eith key k, if any.
   // Then it returns the value previously associated to k in the map, if any.
   // More precisely, it returns Some(v) if k had an associated value v,
   // and returns None otherwhise.
   method remove(k: int) returns (vo: Option<T>)
+  requires isValid()
+  ensures isValid() 
+  modifies this
+  ensures keySet() == old(keySet()) - {k}
+  ensures vo != None ==> (k, vo.val) in old(entrySet())
+  ensures vo == None ==> k !in old(keySet())
+  {
+    vo := get(k);
+    entries := M.remove(entries, k);
+  }
 }
