BubbleSort.dfy
@@ -21,6 +21,7 @@ predicate isSorted(a: array<int>, lo: int, hi: nat)
 // using the bubble sort algorithm
 method BubbleSort(a: array<int>)
   modifies a
+  // requires a.Length >=1
   // a is sorted non-decreasingly at the end
   ensures isSorted(a, 0, a.Length)
   // a is a permutation of old(a) (no elements are added or removed)
@@ -28,15 +29,25 @@ method BubbleSort(a: array<int>)
 {
   var i := a.Length - 1;
   while i > 0
+  decreases i
+  invariant i < a.Length
+  && (forall k :: 0 <= i < k < a.Length  ==> a[k] >= a[i] )
+  && (a.Length > i+1 ==> (forall k :: 0 <= k < (i+1)  ==> a[i+1] >= a[k] ))
+
   {
     var j := 0;
     while j < i
+    decreases i - j
+    invariant j < a.Length && (forall k :: 0 <= k < j  ==> a[j] >= a[k] ) && j <= i
     {
       if a[j] > a[j + 1] {
          a[j], a[j + 1] := a[j + 1], a[j];
       }
       j := j + 1;
-    }    
+    } 
+    assert j == i;
+    assert i < a.Length && (forall k :: 0 <= k < i  ==> a[i] >= a[k] );   
     i := i - 1;
   }
+  assert i >= -1;
 }
